# Copyright 2020  ENERSHARE Project.
# 
# Licensed under the Apache License, Version 2.0 (the "License");
# you may not use this file except in compliance with the License.
# You may obtain a copy of the License at
# 
#      http://www.apache.org/licenses/LICENSE-2.0
# 
# Unless required by applicable law or agreed to in writing,
# distributed under the License is distributed on an "AS IS" BASIS,
# WITHOUT WARRANTIES OR CONDITIONS OF ANY KIND, either express or implied.
# See the License for the specific language governing permissions and
# limitations under the License.

@prefix rdf: <http://www.w3.org/1999/02/22-rdf-syntax-ns#> .
@prefix owl: <http://www.w3.org/2002/07/owl#> .
@prefix rdfs: <http://www.w3.org/2000/01/rdf-schema#> .
@prefix xsd: <http://www.w3.org/2001/XMLSchema#> .
@prefix dcterms: <http://purl.org/dc/terms/> .
@prefix vann: <http://purl.org/vocab/vann/> .
@prefix voaf: <http://purl.org/vocommons/voaf#> .
@prefix vs: <http://www.w3.org/2003/06/sw-vocab-status/ns#> .
@prefix cc: <http://creativecommons.org/ns#>.
@prefix foaf: <http://xmlns.com/foaf/0.1/>.
@prefix seas: <https://w3id.org/seas/> .
@prefix ener: <https://w3id.org/enershare/>.
@prefix sch: <https://schema.org/>.
@prefix fiware:<https://uri.fiware.org/ns/data-models#>.
@prefix ener-rsrc:<https://w3id.org/enershare/energyresource/>.
@prefix ener-bldg: <https://w3id.org/enershare/building/>.
@base <https://w3id.org/enershare/building/>.

voaf:Vocabulary a owl:Class .
dcterms:title a owl:AnnotationProperty .
dcterms:description a owl:AnnotationProperty .
dcterms:issued a owl:AnnotationProperty .
dcterms:modified a owl:AnnotationProperty .
dcterms:creator a owl:AnnotationProperty .
dcterms:contributor a owl:AnnotationProperty .
dcterms:license a owl:AnnotationProperty .
vann:preferredNamespacePrefix a owl:AnnotationProperty .
vann:preferredNamespaceUri a owl:AnnotationProperty .
vs:term_status a owl:AnnotationProperty .
foaf:Person a owl:Class .
foaf:name a owl:DatatypeProperty .

ener-bldg:BuildingyOntology rdf:type voaf:Vocabulary , owl:Ontology ;
  dcterms:title "Enershare Building Ontology"@en ;
  dcterms:description "The Enershare Building vocabulary for the  Enershare  project."@en ;
  dcterms:issued "2024-02-28"^^xsd:date ;
  dcterms:modified "2024-05-30"^^xsd:date ;
  dcterms:creator "Lynda TEMAL, Sarra BEN ABBES and Oumy SEYE";
  dcterms:license <https://www.apache.org/licenses/LICENSE-2.0> ;
  vann:preferredNamespacePrefix "ener-bldg";
  vann:preferredNamespaceUri <https://w3id.org/enershare/building/> ;  
  owl:versionIRI <https://w3id.org/enershare/BuildingOntology-1.1> ;
  owl:inmport <https://w3id.org/seas/BuildingOntology>;
  owl:versionInfo "v1.0".


### https://w3id.org/enershare/building/SingleFamilyHouse
ener-bldg:SingleFamilyHouse a owl:Class ;
  rdfs:label "Single Family House"@en ;
  rdfs:comment """Single Family House is OneDwellingBuilding that is detached house and occuppied by a Single Family"""@en ;
  rdfs:subClassOf seas:OneDwellingBuilding;  
  vs:term_status "testing";
  rdfs:isDefinedBy ener-bldg:BuildingOntology .

### https://w3id.org/enershare/building/MultiDwellingBuilding
ener-bldg:MultiDwellingBuilding a owl:Class ;
  rdfs:label "MultiDwelling Building"@en ;
  rdfs:comment """MultiDwelling Building is a residential building that represents a multiple separate housing units for residential inhabitants are contained 
                  within one building or several buildings within one complex (source: Wikipedia)"""@en ;
  rdfs:subClassOf seas:ResidentalBuilding;  
  vs:term_status "testing";
  rdfs:isDefinedBy ener-bldg:BuildingOntology .

### https://w3id.org/enershare/building/Apartment
ener-bldg:Apartment a owl:Class ;
  skos:altLabel "Flat"@en;
  rdfs:label "Apartment"@en ;
  rdfs:comment """An apartment (North American English), flat (British English, Indian English, South African English)[a], or unit (Australian English) 
                  is a self-contained housing unit (a type of residential real estate) that occupies part of a building, generally on a single storey. (source: Wikipedia) """@en ;
  rdfs:subClassOf seas:ResidentalBuilding;  
  rdfs:subClassOf [ a owl:Restriction ; owl:onProperty seas:subZoneOf ; owl:someValuesFrom ener-bldg:MultiDwellingBuilding] ;
  vs:term_status "testing";
  rdfs:seeAlso fiware:documentation;
  rdfs:isDefinedBy ener-bldg:BuildingOntology .
  
### https://w3id.org/enershare/building/EnergyAuditDocument
ener-bldg:EnergyAuditDocument a owl:Class ;
  rdfs:label "Energy Audit Document"@en ;
  rdfs:comment """Energy Audit Document is a digital document that includ the energy audit of the building"""@en ;
  rdfs:subClassOf sch:DigitalDocument;  
  vs:term_status "testing";
  rdfs:seeAlso fiware:documentation;
  rdfs:isDefinedBy ener-bldg:BuildingOntology .

### https://w3id.org/enershare/building/hasEnergyAuditDocument
ener-bldg:hasEnergyAuditDocument a owl:ObjectProperty , owl:FunctionalProperty ;
  rdfs:label "has Energy Audit Document"@en ;
  rdfs:comment """has Energy Audit Document relates the Building to it Energy audit Document"""@en ;
  rdfs:subPropertyOf seas:hasProperty;
  rdfs:domain seas:Building;
  rdfs:range ener-bldg:EnergyAuditDocument;
  rdfs:seeAlso fiware:documentation;
  vs:term_status "testing";
  rdfs:isDefinedBy ener-bldg:BuildingOntology.

### https://w3id.org/enershare/building/hasMansard
ener-bldg:hasMansard a owl:ObjectProperty, owl:Property;
  rdfs:label "has Mansard"@en ;
  rdfs:comment """ has Mansard relates the building to the boolean to indicate if the building has mansard or not"""@en ;
  rdfs:subPropertyOf seas:hasProperty;
  rdfs:domain seas:Building;
  rdfs:range seas:BooleanProperty ;
  vs:term_status "testing";
  rdfs:isDefinedBy ener-bldg:BuildingOntology.

### https://w3id.org/enershare/building/hasRoofFloor
ener-bldg:hasRoofFloor a owl:ObjectProperty , owl:FunctionalProperty ;
  rdfs:label "has Roof Floor"@en ;
  rdfs:comment """has Roof Floor relates the building to the boolean to indicate if the building has Roof floor or not """@en ;
  rdfs:subPropertyOf seas:hasProperty;
  rdfs:domain seas:Building;
  rdfs:range seas:BooleanProperty ;
  rdfs:seeAlso fiware:rooftop;
  vs:term_status "testing";
  rdfs:isDefinedBy ener-bldg:BuildingOntology.

### https://w3id.org/enershare/building/hasUndergroundFloor 
ener-bldg:hasUndergroundFloor a owl:ObjectProperty , owl:FunctionalProperty ;
  rdfs:label "has Underground Floor"@en ;
  rdfs:comment """has Underground Floor relates the building to the boolean to indicate if the building has Underground Floor or not"""@en ;
  rdfs:subPropertyOf seas:hasProperty;
  rdfs:domain seas:Building;
  rdfs:range seas:BooleanProperty ;
  rdfs:seeAlso fiware:floorsBelowGround;
  vs:term_status "testing";
  rdfs:isDefinedBy ener-bldg:BuildingOntology.

### https://w3id.org/enershare/building/hasWaterHeatingSystem
ener-bldg:hasWaterHeatingSystem a owl:ObjectProperty , owl:FunctionalProperty ;
  rdfs:label "has Water Heating System"@en ;
  rdfs:comment """has Water Heating System relates the building to the boolean to indicate if the building has Water Heating System or not"""@en ;
  rdfs:subPropertyOf seas:hasProperty;
  rdfs:domain seas:Building;
  rdfs:range seas:BooleanProperty ;
  vs:term_status "testing";
  rdfs:isDefinedBy ener-bldg:BuildingOntology.

### https://w3id.org/enershare/building/hasHeatInstallationSystem
ener-bldg:hasHeatInstallationSystem a owl:ObjectProperty , owl:FunctionalProperty ;
  rdfs:label "has Heat Installation System"@en ;
  rdfs:comment """has Heat Installation System relates the building to the boolean to indicate if the building has Heat Installation System or not"""@en ;
  rdfs:subPropertyOf seas:hasProperty;
  rdfs:domain seas:Building;
  rdfs:range seas:BooleanProperty ;
  vs:term_status "testing";
  rdfs:isDefinedBy ener-bldg:BuildingOntology.

### https://w3id.org/enershare/building/hasCoolingSystem
ener-bldg:hasCoolingSystem a owl:ObjectProperty , owl:FunctionalProperty ;
  rdfs:label "has Cooling System"@en ;
  rdfs:comment """has Cooling System relates the building to the boolean to indicate if the building is equipped with cooling system."""@en ;
  rdfs:subPropertyOf seas:hasProperty;
  rdfs:domain seas:Building;
  rdfs:range seas:BooleanProperty ;
  vs:term_status "testing";
  rdfs:isDefinedBy ener-bldg:BuildingOntology.  

### https://w3id.org/enershare/building/hasMicroGenerationSystem 
ener-bldg:hasMicroGenerationSystem a owl:ObjectProperty , owl:FunctionalProperty ;
  rdfs:label "has Micro Generation System" @en ;
  rdfs:comment """has Micro Generation System relates the building to the boolean to indicate if the building is equipped with micro generation system."""@en ;
  rdfs:subPropertyOf seas:hasProperty;
  rdfs:domain seas:Building;
  rdfs:range seas:BooleanProperty ;
  vs:term_status "testing";
  rdfs:isDefinedBy ener-bldg:BuildingOntology.   

### https://w3id.org/enershare/building/hasCarryingOutConstructionWorks
ener-bldg:hasCarryingOutConstructionWorks a owl:ObjectProperty , owl:FunctionalProperty ;
  rdfs:label "has Carrying Out Construction Works"@en ;
  rdfs:comment """has Carrying Out Construction Works relates the building to the boolean to indicate if the building has Carrying Out Construction Works or not"""@en ;
  rdfs:subPropertyOf seas:hasProperty;
  rdfs:domain seas:Building;
  rdfs:range seas:BooleanProperty ;
  vs:term_status "testing";
  rdfs:isDefinedBy ener-bldg:BuildingOntology.

### https://w3id.org/enershare/building/hasReconstructionOfEnergeeringSystems 
ener-bldg:hasReconstructionOfEnergeeringSystems a owl:ObjectProperty , owl:FunctionalProperty ;
  rdfs:label "has Reconstruction Of Energeering Systems"@en ;
  rdfs:comment """has Reconstruction Of Energeering Systems relates the building to the boolean to indicate if the building has Reconstruction Of Energeering Systems or not"""@en ;
  rdfs:subPropertyOf seas:hasProperty;
  rdfs:domain seas:Building;
  rdfs:range seas:BooleanProperty ;
  vs:term_status "testing";
  rdfs:isDefinedBy ener-bldg:BuildingOntology.

### https://w3id.org/enershare/building/isAlmostZeroEnergyBuilding
ener-bldg:isAlmostZeroEnergyBuilding a owl:ObjectProperty , owl:FunctionalProperty ;
  rdfs:label "is Almost Zero Energy Building"@en ;
  rdfs:comment """is Almost Zero Energy Building relates the building to the boolean to indicate if the building is Almost Zero Energy Building or not"""@en ;
  rdfs:subPropertyOf seas:hasProperty;
  rdfs:domain seas:Building;
  rdfs:range seas:BooleanProperty ;
  vs:term_status "testing";
  rdfs:isDefinedBy ener-bldg:BuildingOntology.

### https://w3id.org/enershare/building/hasFirstEnergyResourceForHeating
ener-bldg:hasFirstEnergyResourceForHeating a owl:ObjectProperty , owl:FunctionalProperty ;
  rdfs:label  "has First Energy Resource For Heating"@en ;
  rdfs:comment """has First Energy Resource For Heating relates the building to it Energy Resource Type"""@en ;
  rdfs:subPropertyOf seas:hasProperty;
  rdfs:domain seas:Building;
  rdfs:range ener-rsrc:EnergyResourceType ;
  vs:term_status "testing";
  rdfs:isDefinedBy ener-bldg:BuildingOntology.

### https://w3id.org/enershare/building/hasSecondEnergyResourceForHeating 
ener-bldg:hasSecondEnergyResourceForHeating a owl:ObjectProperty , owl:FunctionalProperty ;
  rdfs:label  "has Second Energy Resource For Heating"@en ;
  rdfs:comment """has Second Energy Resource For Heating relates the building to it Energy Resource Type """@en ;
  rdfs:subPropertyOf seas:hasProperty;
  rdfs:domain seas:Building;
  rdfs:range ener-rsrc:EnergyResourceType ;
  vs:term_status "testing";
  rdfs:isDefinedBy ener-bldg:BuildingOntology.

### https://w3id.org/enershare/building/hasFirstEnergyResourceForCooling
ener-bldg:hasFirstEnergyResourceForCooling a owl:ObjectProperty , owl:FunctionalProperty ;
  rdfs:label  "has First Energy Resource For Cooling"@en ;
  rdfs:comment """has First Energy Resource For Cooling relates the building to it Energy Resource Type"""@en ;
  rdfs:subPropertyOf seas:hasProperty;
  rdfs:domain seas:Building;
  rdfs:range ener-rsrc:EnergyResourceType ;
  vs:term_status "testing";
  rdfs:isDefinedBy ener-bldg:BuildingOntology.

### https://w3id.org/enershare/building/hasSecondEnergyResourceForCooling 
ener-bldg:hasSecondEnergyResourceForCooling a owl:ObjectProperty , owl:FunctionalProperty ;
  rdfs:label  "has Second Energy Resource For Cooling"@en ;
  rdfs:comment """has Second Energy Resource For Cooling relates the building to it Energy Resource Type"""@en ;
  rdfs:subPropertyOf seas:hasProperty;
  rdfs:domain seas:Building;
  rdfs:range ener-rsrc:EnergyResourceType ;
  vs:term_status "testing";
  rdfs:isDefinedBy ener-bldg:BuildingOntology.

### https://w3id.org/enershare/building/hasFirstEnergyResourceForHotWater
ener-bldg:hasFirstEnergyResourceForHotWater a owl:ObjectProperty , owl:FunctionalProperty ;
  rdfs:label  "has First Energy Resource For Hot Water"@en ;
  rdfs:comment """has First Energy Resource For Hot Water relates the building to it Energy Resource Type"""@en ;
  rdfs:subPropertyOf seas:hasProperty;
  rdfs:domain seas:Building;
  rdfs:range ener-rsrc:EnergyResourceType ;
  vs:term_status "testing";
  rdfs:isDefinedBy ener-bldg:BuildingOntology.

### https://w3id.org/enershare/building/hasSecondEnergyResourceForHotWater 
ener-bldg:hasSecondEnergyResourceForHotWater a owl:ObjectProperty , owl:FunctionalProperty ;
  rdfs:label  "has Second Energy Resource For Hot Water"@en ;
  rdfs:comment """has Second Energy Resource For Hot Water relates the building to it Energy Resource Type"""@en ;
  rdfs:subPropertyOf seas:hasProperty;
  rdfs:domain seas:Building;
  rdfs:range ener-rsrc:EnergyResourceType ;
  vs:term_status "testing";
  rdfs:isDefinedBy ener-bldg:BuildingOntology.

### https://w3id.org/enershare/building/hasEnergyResourceForVentilation
ener-bldg:hasEnergyResourceForVentilation a owl:ObjectProperty , owl:FunctionalProperty ;
  rdfs:label  "has Second Energy Resource For Hot Water"@en ;
  rdfs:comment """has Second Energy Resource For Hot Water relates the building to it Energy Resource Type"""@en ;
  rdfs:subPropertyOf seas:hasProperty;
  rdfs:domain seas:Building;
  rdfs:range ener-rsrc:EnergyResourceType ;
  vs:term_status "testing";
  rdfs:isDefinedBy ener-bldg:BuildingOntology.


### https://w3id.org/enershare/building/hasVentilationEfficiency
ener-bldg:hasVentilationEfficiency a owl:DatatypeProperty ;
  rdfs:label  "has Ventilation Efficiency"@en ;
  rdfs:comment """"""@en ;
  rdfs:domain seas:Building;
  rdfs:range seas:EfficiencyProperty;
  vs:term_status "testing";
  rdfs:isDefinedBy ener-bldg:BuildingOntology.


### https://w3id.org/enershare/building/hasNumberOfResidents
ener-bldg:hasNumberOfResidents a owl:DatatypeProperty ;
  rdfs:label  "has Number Of Residents"@en ;
  rdfs:comment """Number Of People living in the building"""@en ;
  rdfs:domain seas:Building;
  rdfs:range xsd:integer ;
  vs:term_status "testing";
  rdfs:isDefinedBy ener-bldg:BuildingOntology.


### https://w3id.org/enershare/building/hasNumberOfFloors
ener-bldg:hasNumberOfFloors a owl:DatatypeProperty ;
  rdfs:label  "has Number Of Floors"@en ;
  rdfs:comment """Number Of Floors of a building"""@en ;
  rdfs:domain seas:Building;
  rdfs:range xsd:integer ;
  vs:term_status "testing";
  rdfs:isDefinedBy ener-bldg:BuildingOntology.


### https://w3id.org/enershare/building/hasNumberOfFloors
ener-bldg:hasNumberOfBuildings a owl:DatatypeProperty ;
  rdfs:label  "has Number Of Buildings"@en ;
  rdfs:comment """Number Of Buildings in a zone"""@en ;
  rdfs:range xsd:integer ;
  vs:term_status "testing";
  rdfs:isDefinedBy ener-bldg:BuildingOntology.



### https://w3id.org/enershare/building/hasNumberOfUndergroundFloors
ener-bldg:hasNumberOfUndergroundFloors a owl:DatatypeProperty ;
  rdfs:label  "has Number Of Underground Floors"@en ;
  rdfs:comment """Number Of Underground Floors of a building"""@en ;
  rdfs:domain seas:Building;
  rdfs:range xsd:integer ;
  vs:term_status "testing";
  rdfs:isDefinedBy ener-bldg:BuildingOntology.  


#####################################
# Overall heat transfer coefficient # 
#####################################

### https://w3id.org/enershare/building/OverallHeatTransferCoefficientProperty
ener-bldg:OverallHeatTransferCoefficientProperty a owl:Class ;
  rdfs:label "Overall heat transfer coefficient Property"@en ;
  rdfs:comment """The overall heat transfer coefficient {displaystyle U} U is a measure of the overall ability of a series of conductive and 
                  convective barriers to transfer heat. It is commonly applied to the calculation of heat transfer in heat exchangers, 
                  but can be applied equally well to other problems.(source:wikipedia)"""@en ;
  rdfs:subClassOf seas:Property ;
  vs:term_status "testing" ;
  rdfs:isDefinedBy ener-bldg:BuildingOntology. 

### https://w3id.org/enershare/building/OverallHeatTransferCoefficientEvaluation
ener-bldg:OverallHeatTransferCoefficientEvaluation a owl:Class ;
  rdfs:label "Overall heat transfer coefficient Evaluation"@en ;
  rdfs:comment """The class Overall heat transfer coefficient evaluation for Overall heat transfer coefficient properties"""@en ;
  rdfs:subClassOf seas:Evaluation ;
  rdfs:subClassOf [ owl:onProperty seas:evaluationOf ; owl:someValuesFrom ener-bldg:OverallHeatTransferCoefficientProperty ] ;
  owl:equivalentClass [ owl:onProperty seas:evaluationOf ; owl:someValuesFrom ener-bldg:OverallHeatTransferCoefficientProperty ] ;
  vs:term_status "testing" ;
  rdfs:isDefinedBy ener-bldg:BuildingOntology.

### https://w3id.org/enershare/building/hasOverallHeatTransferCoefficient
ener-bldg:hasOverallHeatTransferCoefficient a owl:ObjectProperty , owl:FunctionalProperty ;
  rdfs:label "overall heat transfer coefficient"@en ;
  rdfs:comment """Links the building to its overall heat transfer coefficient property."""@en ;
  rdfs:subPropertyOf seas:hasProperty ;
  rdfs:domain seas:Building ;
  rdfs:range ener-bldg:OverallHeatTransferCoefficientProperty ;
  vs:term_status "testing" ;
  rdfs:isDefinedBy ener-bldg:BuildingOntology. 

## https://w3id.org/enershare/building/hasOverallHeatTransferCoefficientThroughVerticalWall
ener-bldg:hasOverallHeatTransferCoefficientThroughVerticalWall a owl:ObjectProperty , owl:FunctionalProperty ;
  rdfs:label "overall heat transfer coefficient through vertical wall"@en ;
  rdfs:comment """Overall heat transfer coefficient in W/m²K. It represents the heat flux transfer through a wall, 
                  normalized by the wall surface and the difference of temperature across the wall, at steady state."""@en ;
  rdfs:subPropertyOf ener-bldg:hasOverallHeatTransferCoefficient ;
  rdfs:domain seas:Building ;
  rdfs:range ener-bldg:OverallHeatTransferCoefficientProperty ;
  vs:term_status "testing" ;
  rdfs:isDefinedBy ener-bldg:BuildingOntology. 

## https://w3id.org/enershare/building/hasOverallHeatTransferCoefficientThroughRoof
ener-bldg:hasOverallHeatTransferCoefficientThroughRoof a owl:ObjectProperty , owl:FunctionalProperty ;
  rdfs:label "overall heat transfer coefficient through roof"@en ;
  rdfs:comment """Overall heat transfer coefficient in W/m²K. It represents the heat flux transfer through a roof, 
                normalized by the roof surface and the difference of temperature across the roof, at steady state.."""@en ;
  rdfs:subPropertyOf ener-bldg:hasOverallHeatTransferCoefficient ;
  rdfs:domain seas:Building ;
  rdfs:range ener-bldg:OverallHeatTransferCoefficientProperty ;
  vs:term_status "testing" ;
  rdfs:isDefinedBy ener-bldg:BuildingOntology. 

## https://w3id.org/enershare/building/hasOverallHeatTransferCoefficientThroughFloor
ener-bldg:hasOverallHeatTransferCoefficientThroughFloor a owl:ObjectProperty , owl:FunctionalProperty ;
rdfs:label "overall heat transfer coefficient through floor"@en ;
rdfs:comment """Overall heat transfer coefficient in W/m²K. It represents the heat flux transfer through a floor, 
              normalized by the floor surface and the difference of temperature across the floor, at steady state."""@en ;
rdfs:subPropertyOf ener-bldg:hasOverallHeatTransferCoefficient ;
rdfs:domain seas:Building ;
rdfs:range ener-bldg:OverallHeatTransferCoefficientProperty ;
vs:term_status "testing" ;
rdfs:isDefinedBy ener-bldg:BuildingOntology. 

## https://w3id.org/enershare/building/hasOverallHeatTransferCoefficientThroughOpening
ener-bldg:hasOverallHeatTransferCoefficientThroughOpening a owl:ObjectProperty , owl:FunctionalProperty ;
rdfs:label "overall heat transfer coefficient through opening"@en ;
rdfs:comment """Overall heat transfer coefficient in W/m²K. It represents the heat flux transfer through an opening, 
              normalized by the opening surface and the difference of temperature across the opening, at steady state."""@en ;
rdfs:subPropertyOf ener-bldg:hasOverallHeatTransferCoefficient ;
rdfs:domain seas:Building ;
rdfs:range ener-bldg:OverallHeatTransferCoefficientProperty ;
vs:term_status "testing" ;
rdfs:isDefinedBy ener-bldg:BuildingOntology. 
